Almost there on BrD

theories/CTree/Logic/AF.v
@@ -91,24 +91,17 @@ Section BasicLemmas.
         apply ktrans_brD in H0 as (i & TR).
         destruct (H i); eauto.
   Qed.
-
-  Lemma can_step_stuck: forall w,
-      can_step (Ctree.stuck: ctree E X) w -> False.
-  Proof.
-    intros w (t' & w' & TR).
-    cbn in TR.
-    dependent induction TR; eauto.
-  Qed.
   
   Lemma af_stuck: forall w φ,
-      <( {Ctree.stuck: ctree E X}, w |= AF now φ )> ->
+      <( {Ctree.stuck: ctree E X}, w |= AF now φ )> <->
       φ w.
   Proof.
-    intros.
-    cbn in H; dependent induction H; auto.
-    destruct H0, H1.
-    apply can_step_stuck in H1.
-    contradiction.
+    split; intros.
+    - cbn in H; dependent induction H; auto.
+      destruct H0, H1.
+      apply can_step_stuck in H1.
+      contradiction.
+    - now next; left.
   Qed.
   
   Lemma af_brS: forall n (k: fin' n -> ctree E X) w φ,
@@ -153,10 +146,393 @@ Section BasicLemmas.
 
 End BasicLemmas.
 
+Section AfDoneIndLemma.
+  Context {E: Type} {HE: Encode E} {X: Type}.
+
+  (* t |= AF AX done R *)
+  Inductive AFDoneInd(φ: X -> World E -> Prop): ctree E X -> World E -> Prop :=
+  | AFDoneDone: forall t (x: X),
+      observe t = RetF x ->
+      φ x Pure ->
+      AFDoneInd φ t Pure
+  | AFDoneFinish: forall t (e: E) (v: encode e) (x: X),
+      observe t = RetF x ->
+      φ x (Obs e v) ->
+      AFDoneInd φ t (Obs e v)
+  | AFDoneBr: forall b n t (k: fin' n -> ctree E X) w,
+      observe t = BrF b n k ->
+      not_done w ->
+      (forall (i: fin' n), AFDoneInd φ (k i) w) ->
+      AFDoneInd φ t w
+  |AFDoneVis: forall (t: ctree E X) w e k,
+      observe t = VisF e k ->
+      not_done w ->
+      (forall (v: encode e), AFDoneInd φ (k v) (Obs e v)) ->
+      AFDoneInd φ t w.
+  
+  Global Instance proper_equ_afdoneind φ:
+    Proper (equ eq ==> eq ==> iff) (AFDoneInd φ).
+  Proof.
+    unfold Proper, respectful.
+    intros; subst; split; intros Hind.
+    - generalize dependent y.
+      induction Hind; intros.
+      + apply AFDoneDone with x; auto.
+        rewrite <- H.
+        unfold equ in H.
+        step in H1; cbn in H1; dependent destruction H1;
+          congruence.
+      + apply AFDoneFinish with x; auto.
+        rewrite <- H.
+        step in H1; cbn in H1; dependent destruction H1;
+          congruence.
+      + unfold equ; step in H3; cbn in H3; rewrite H in H3.
+        dependent destruction H3.
+        apply AFDoneBr with b n k2; auto; intros.
+        apply H2 with i, H3.
+      + unfold equ; step in H3; cbn in H3; rewrite H in H3.
+        dependent destruction H3.
+        eapply AFDoneVis with e k2; auto; intros.
+        apply H2, H3.
+    - generalize dependent x.
+      induction Hind; intros.
+      + apply AFDoneDone with x; auto.
+        rewrite <- H.
+        unfold equ in H.
+        step in H1; cbn in H1; dependent destruction H1;
+          congruence.
+      + apply AFDoneFinish with x; auto.
+        rewrite <- H.
+        step in H1; cbn in H1; dependent destruction H1;
+          congruence.
+      + unfold equ; step in H3; cbn in H3; rewrite H in H3.
+        dependent destruction H3.
+        apply AFDoneBr with b n k1; auto; intros.
+        apply H2 with i, H3.
+      + unfold equ; step in H3; cbn in H3; rewrite H in H3.
+        dependent destruction H3.
+        eapply AFDoneVis with e k1; auto; intros.
+        apply H2, H3.
+  Qed.
+
+  Lemma afdoneind_stuck: forall w φ,
+      ~ (AFDoneInd φ Ctree.stuck w).
+  Proof.
+    intros * Hcontra.
+    dependent induction Hcontra; eauto.
+    cbn in x.
+    dependent destruction x.
+    apply H2; auto.
+    exact (Fin.F1).
+  Qed.
+
+  Lemma afdone_step_done (t t': ctree E X) (w w': World E) φ : forall x,
+      [t, w] ↦ [t', Done x] ->      
+      φ x Pure ->
+      w = Pure /\ AFDoneInd φ t w.
+  Proof.
+    intros x TR; cbn in TR.
+    dependent induction TR; intros; split.
+    - now destruct (IHTR _ _ x0 eq_refl eq_refl eq_refl H).
+    - apply AFDoneBr with false n k; auto.
+      + now apply ktrans_not_done with (k i) t'0 (Done x0).
+      + admit.
+  Admitted.
+
+  Lemma afdone_step_finish (t t': ctree E X) (w w': World E) φ : forall (e: E) (v: encode e) x,
+      [t, w] ↦ [t', Finish e v x] ->      
+      φ x (Obs e v) ->
+      w = Obs e v /\ AFDoneInd φ t w.
+  Proof.
+  Admitted.
+
+  Lemma afdone_ind: forall φ (t: ctree E X) w,
+      <( t, w |= AF AX done φ )> ->
+      AFDoneInd φ t w.
+  Proof.
+    intros; induction H.
+    - (* now *)
+      next in H.
+      destruct H as [(t_ & w_ & TR_) H].
+      cbn in TR_, H.
+      desobs t.
+      + (* Ret *)
+        pose proof (ktrans_not_done (Ret x) t_ w w_ TR_).
+        inv H0.
+        * (* Ret, Pure *)
+          apply AFDoneDone with x; auto.
+          specialize (H _ _ TR_).
+          dependent destruction TR_; dependent destruction H; auto.
+        * (* Ret, Obs *)
+          apply AFDoneFinish with x; auto.
+          specialize (H _ _ TR_).
+          dependent destruction TR_; dependent destruction H; auto.
+      + (* Br *)
+        apply AFDoneBr with b n k; auto.
+        * now apply ktrans_not_done with (Br b n k) t_ w_.
+        * destruct b.
+          -- (* BrS *)
+            intros v'.
+            specialize (H _ _ TR_).
+            dependent destruction TR_; dependent destruction H1; inv H.
+          -- (* BrD *)
+            setoid_rewrite ktrans_brD in H.
+            apply ktrans_brD in TR_ as (i & TR_).
+            rewrite pull2_iff in H.
+            clear Heqt t.
+            (* things are looking reasonable at this point! *)
+            generalize dependent k.
+            revert i.
+            revert t_ w_ w φ.
+            induction n; intros.
+            ++ dependent destruction i0; try solve [inv i0].
+               dependent destruction i; try solve [inv i].
+               specialize (H _ _ Fin.F1 TR_).
+               dependent destruction H.
+               ** apply afdone_step_done with
+                    (t:=k Fin.F1) (w:=w) (t':=t_) (x:=x) (φ:=φ) in TR_;
+                    intuition.
+               ** apply afdone_step_finish with
+                    (t:=k Fin.F1) (w:=w) (t':=t_) (x:=x) (φ:=φ) in TR_;
+                    intuition.
+            ++ admit.
+      + (* Vis *)
+        apply AFDoneVis with e k; eauto.
+        * now apply ktrans_not_done with (Vis e k) t_ w_.
+        * intros v'.
+          specialize (H _ _ TR_).
+          dependent destruction TR_; dependent destruction H1; inv H.
+    - (* AX AF *)
+      destruct H0, H1.
+      clear H H1.
+      destruct H0 as (t_ & w_ & TR_).
+      cbn in TR_, H2, H3.
+      desobs t.
+      + (* Ret *)
+        pose proof (ktrans_not_done (Ret x) t_ w w_ TR_).
+        inv H.
+        * (* Ret, Pure *)
+          apply AFDoneDone with x; auto.
+          specialize (H3 _ _ TR_).
+          dependent destruction TR_; dependent destruction H3; inv H0.
+        * (* Ret, Obs *)
+          apply AFDoneFinish with x; auto.
+          specialize (H3 _ _ TR_).
+          dependent destruction TR_; dependent destruction H3; inv H0.
+      + (* Br *)
+        apply AFDoneBr with b n k; auto.
+        * now apply ktrans_not_done with (Br b n k) t_ w_.
+        * destruct b.
+          -- (* BrS *)
+            intros v'.
+            specialize (H2 _ _ TR_).
+            apply H3; econstructor; auto.
+            now apply ktrans_not_done with (Br true n k) t_ w_.
+          -- (* BrD *)
+            setoid_rewrite ktrans_brD in H2.
+            setoid_rewrite ktrans_brD in H3.
+            apply ktrans_brD in TR_ as (i & TR_).
+            rewrite pull2_iff in H2, H3.
+            (* things are looking reasonable at this point! *)
+            admit.
+      + (* Vis *)
+        apply AFDoneVis with e k; eauto.
+        * now apply ktrans_not_done with (Vis e k) t_ w_.
+        * intros v'.
+          specialize (H2 _ _ TR_).
+          dependent destruction TR_; dependent destruction H2; apply H3; econstructor; auto.
+  Admitted.
+
+  Lemma af_ret_inv: forall (x: X) w R,
+      <( {Ret x}, w |= AF (AX done R) )> ->
+      R x w.
+  Proof.
+    intros.
+    apply afdone_ind in H.
+    dependent induction H; auto.
+  Qed.
+
+End AfDoneIndLemma.
+
+Section CtlAfBind.
+  Context {E: Type} {HE: Encode E}.
+
+  Typeclasses Transparent equ.
+  Theorem af_bind_vis{X Y}: forall (t: ctree E Y) (k: Y -> ctree E X) φ w,
+      <( t, w |= AF vis φ )> ->
+      <( {x <- t ;; k x}, w |= AF vis φ )>.
+  Proof.
+    intros * Haf.
+    revert X k.
+    induction Haf; intros; subst.
+    - (* MatchA *)
+      next; left; cbn; destruct H as (e_ & x_ & ? & ?); subst.
+      now (exists e_, x_).
+    - (* StepA *)
+      destruct H0, H1; clear H H0.
+      destruct H1 as (t_ & w_ & TR_).
+      next; right; next; split.
+      * eapply can_step_bind_l; eauto.
+  Admitted.
+
+  Theorem af_bind_pure{X Y}: forall (t: itree E Y) (k: Y -> itree E X) w,
+      <( t, w |= AF pure )> ->
+      <( {x <- t ;; k x}, w |= AF pure )>.
+  Proof.
+    intros * Haf.
+    apply af_afind in Haf.
+    revert X k.    
+    induction Haf; intros; subst. 
+    - (* Base *)
+      next; left; now cbn. 
+    - (* Done *)
+      inv H0.
+    - (* Finish *)
+      inv H0.
+    - (* Tau *)
+      observe_equ H.
+      rewrite Eqt, bind_tau.
+      apply af_tau; eauto.
+    - (* Vis *)
+      observe_equ H.
+      rewrite Eqt, bind_vis.
+      apply af_vis; eauto.
+  Qed.
+  
+  Lemma can_step_bind_r{X Y}: forall (t: itree E Y) (k: Y -> itree E X) w R,      
+      <( t, w |= AF AX done R )> ->
+      (forall y w, R y w -> can_step (k y) w) ->
+      can_step (x <- t ;; k x) w.
+  Proof.    
+    intros.
+    apply afdone_ind in H.
+    generalize dependent k.
+    induction H; intros; observe_equ H; rewrite Eqt.
+    - (* Done x *)
+      rewrite bind_ret_l.
+      now apply H1.
+    - (* Finish *)
+      rewrite bind_ret_l.
+      now apply H1.
+    - (* Tau *)
+      rewrite bind_tau.
+      apply can_step_tau; eauto.
+    - (* Vis *)
+      rewrite bind_vis.
+      apply can_step_vis; auto.
+  Qed.
+  Hint Resolve can_step_bind_r: ctl.
+
+  Theorem af_bind_r{X Y}: forall (t: itree E Y)
+                            (k: Y -> itree E X) w φ R,
+      <( t, w |= AF AX done R )> ->
+      (forall (y: Y) w, R y w -> not_done w ->
+                   <( {k y}, w |= AF now φ )>) ->
+      <( {x <- t ;; k x}, w |= AF now φ )>.
+  Proof.
+    intros.
+    apply afdone_ind in H.
+    revert H0.
+    generalize dependent φ.
+    generalize dependent k.
+    induction H; intros; observe_equ H; rewrite Eqt.
+    - (* Done *)
+      rewrite bind_ret_l; eauto with ctl.
+    - (* Finish *)
+      rewrite bind_ret_l; eauto with ctl.
+    - (* Tau *)
+      rewrite bind_tau.
+      apply af_tau; eauto with ctl.
+    - (* Vis *)
+      rewrite bind_vis.
+      apply af_vis; eauto with ctl.
+  Qed.
+
+End CtlAfBind.
+
+Section CtlAfIter.
+  Context {E: Type} {HE: Encode E}.
+
+  (* Total correctness lemma for [iter] *)
+  (* [Ri: I -> World E -> Prop] loop invariant (left).
+     [Rr: X -> World E -> Prop] loop postcondition (right).
+     [Rv: (I * World E) -> (I * World E) -> Prop)] loop variant (left). *)
+  Lemma af_iter{X I} Ri Rr (Rv: relation (I * World E)) (i: I) w (k: I -> itree E (I + X)):
+      (forall (i: I) w, Ri i w ->
+                   <( {k i}, w |= AF AX done {fun (x: I + X) w' =>
+                                             match x with
+                                             | inl i' => Ri i' w' /\ Rv (i', w') (i, w)
+                                             | inr r' => Rr r' w'
+                                             end})>) ->
+      well_founded Rv ->
+      Ri i w ->
+      <( {Itree.iter k i}, w |= AF done Rr )>.
+  Proof.      
+    intros H WfR Hi.
+    generalize dependent k.
+    revert Hi.
+    remember (i, w) as P.
+    replace i with (fst P) by now subst.
+    replace w with (snd P) by now subst.
+    clear HeqP i w.
+    Opaque entailsF.
+    induction P using (well_founded_induction WfR); (* wf_ind *)
+      destruct P as (i, w); cbn in *. 
+    rename H into HindWf.
+    intros.
+    rewrite unfold_iter.
+    eapply af_bind_r with (R:=fun (x : I + X) (w' : World E) =>
+                                match x with
+                                | inl i' => Ri i' w' /\ Rv (i', w') (i, w)
+                                | inr r' => Rr r' w'
+                                end); auto.
+    intros [i' | r] w'.
+    - intros (Hi' & Hv) Hd.
+      apply af_tau.
+      remember (i', w') as y.
+      replace i' with (fst y) by now subst.
+      replace w' with (snd y) by now subst.      
+      apply HindWf; inv Heqy; auto.
+    - intros Hr Hd.
+      next; right; next; split.
+      + now apply can_step_ret.
+      + intros t_ w_ TR_.
+        inv Hd.
+        * apply ktrans_pure in TR_ as (-> & ->).
+          next; left.
+          rewrite ctl_done.
+          now constructor.
+        * apply ktrans_finish in TR_ as (-> & ->).
+          next; left.
+          rewrite ctl_done.
+          now constructor.          
+  Qed.
+End CtlAfIter.
+
 Section AfIndLemma.
   Context {E: Type} {HE: Encode E} {X: Type}.
 
-  (* t, w |= WF now φ *)
+  (* t |= AX AF done R *)
+  Inductive AXAFInd(φ: World E -> Prop): ctree E X -> World E -> Prop :=
+  | AXAFDoneBase: forall t (x: X),
+      observe t = RetF x ->
+      φ Ctree.stuck (Done x) ->
+      AXAFDoneInd t Pure
+  | AXAFFinishBase: forall t (e: E) (v: encode e) (x: X),
+      observe t = RetF x ->
+      φ Ctree.stuck (Finish e v x) ->
+      AXAFDoneInd t (Obs e v)
+  | AXAFBrD: forall t u w,
+      observe t = BrF b n k ->
+      (forall (i: fin' n), AFDoneInd (k i) w) ->
+      AFDoneInd t w
+  |AFDoneIndVis: forall (t: itree E X) w e k (_: encode e),
+      observe t = VisF e k ->
+      not_done w ->
+      (forall (v: encode e), AFDoneInd (k v) (Obs e v)) ->
+      AFDoneInd t w.
+
+  (* t, w |= AX AF now φ *)
   Inductive AFNowInd(φ: World E -> Prop): ctree E X -> World E -> Prop :=
   | AFNowIndBase: forall (t: ctree E X) (w: World E),
       φ w ->
@@ -169,10 +545,16 @@ Section AfIndLemma.
       observe t = RetF x ->
       φ (Finish e v x) ->
       AFNowInd φ t (Obs e v)
-  | AFNowIndBr: forall t w b n (k: fin' n -> ctree E X),
-      observe t = BrF b n k ->
+  | AFNowIndBrS: forall t w n (k: fin' n -> ctree E X),
+      observe t = BrF true n k ->
       not_done w ->
-      (forall (i: fin' n), can_step (k i) w -> AFNowInd φ (k i) w) ->
+      (forall (i: fin' n), AFNowInd φ (k i) w) ->
+      AFNowInd φ t w
+  | AFNowIndBrD: forall t t' w w' n (k: fin' n -> ctree E X),
+      observe t = BrF false n k ->
+      not_done w ->
+      (exists i, can_step (k i) w) ->
+      (forall (i: fin' n), [k i, w] ↦ [t', w'] -> AFNowInd φ t' w') ->
       AFNowInd φ t w
   | AFNowIndVis: forall (t: ctree E X) w e k,
       observe t = VisF e k ->
@@ -194,92 +576,19 @@ Section AfIndLemma.
       + apply AFNowIndFinish with x; auto.
         unfold equ in H1; step in H1; cbn in H1;
           dependent destruction H1; congruence.
-      + step in H3; cbn in H3; rewrite H in H3.
-        dependent destruction H3.
-        eapply AFNowIndBr with b n k2; auto.
-        intros i (t' & w' & TR').
-        eapply H2 with i; [|apply H3].
-        assert (Heqi: k i ≅ k2 i) by apply H3; auto.
-        rewrite Heqi. 
-        now (exists t', w').
-      + step in H3; cbn in H3; rewrite H in H3.
-        dependent destruction H3.
-        eapply AFNowIndVis with e k2; auto.
-        intros.
-        apply H2, H3.
-    - generalize dependent x.
-      induction Hind; intros.
-      + apply AFNowIndBase; auto.        
-      + apply AFNowIndDone with x; auto.
-        unfold equ in H1; step in H1; cbn in H1;
-          dependent destruction H1; congruence.
-      + apply AFNowIndFinish with x; auto.
-        unfold equ in H1; step in H1; cbn in H1;
-          dependent destruction H1; congruence.
-      + step in H3; cbn in H3; rewrite H in H3.
-        dependent destruction H3.
-        eapply AFNowIndBr with b n k1; auto.
-        intros i (t' & w' & TR').
-        assert (Heqi: k1 i ≅ k i) by apply H3; auto.
-        eapply H2 with i; auto.
-        rewrite <- Heqi.
-        now (exists t', w').
-      + step in H3; cbn in H3; rewrite H in H3.
-        dependent destruction H3.
-        eapply AFNowIndVis with e k1; auto.
-        intros.
-        apply H2, H3.
-  Qed.
+  Admitted.
 
   Lemma afind_stuck: forall w φ,
       AFNowInd φ (Ctree.stuck: ctree E X) w -> φ w.
   Proof.
     intros.
     Transparent Ctree.stuck.
-    remember (Ctree.stuck) as S.
-    induction H; intros; subst; auto; unfold Ctree.stuck in H; dependent destruction H.
-  Abort.
-
-  Lemma afind_brD_aux: forall n (k: fin' n -> ctree E X) w φ,
-      (forall i, AFNowInd φ (k i) w) ->
-      φ w \/ (forall i, can_step (k i) w /\
-                    (forall t' w', [k i, w] ↦ [t', w'] ->
-                              AFNowInd φ t' w')).
-  Proof.
-    induction n; intros.
-    - specialize (H Fin.F1).
-      dependent induction H.
-      + (* AFIndNow *) now left.
-      + (* AFIndDone *)
-        right; intros.
-        dependent destruction i; try solve [inv i].
-        split; unfold can_step; cbn; rewrite H.
-        * exists Ctree.stuck, (Done x).
-          now econstructor.
-        * intros * TR.
-          dependent destruction TR.
-          now apply AFNowIndBase.
-      + (* AFIndFinish *)
-        right; intros.
-        dependent destruction i; try solve [inv i].
-        split; unfold can_step; cbn; rewrite H.
-        * exists Ctree.stuck, (Finish e v x).
-          now econstructor.
-        * intros * TR.
-          dependent destruction TR.
-          now apply AFNowIndBase.
-      + (* AFIndBr *) destruct b.
-        * (* BrS *) right.
-          intro i.
-          dependent destruction i; try solve [inv i].
-          unfold can_step; cbn; setoid_rewrite H.
-          split; intros.
-          -- exists (k0 Fin.F1), w; try econstructor; auto.
-          -- admit. 
-        * (* BrD *)
-          induction n.
-          -- edestruct H2.
-  Admitted.
+    dependent induction H; auto.
+    - cbn in x.
+      dependent destruction x.
+      destruct H1.
+      now apply can_step_stuck in H.
+  Qed.
 
   Lemma pull1_iff: forall {A B} (P : A -> Prop) (R : A -> B -> Prop),
       (forall a, (exists b, R a b)-> P a) <-> (forall a b, R a b -> P a).
@@ -306,38 +615,55 @@ Section AfIndLemma.
     induction H.
     - now apply AFNowIndBase.
     - destruct H0, H1; clear H H1.
-      destruct H0 as (t' & w' & TR).      
-      cbn in TR; desobs t. 
+      rewrite ctree_eta in H0; rewrite ctree_eta; cbn in H2, H3.
+      destruct H0 as (t_ & w_ & TR_); cbn in TR_.
+      desobs t; [|destruct b | ].
       + (* RetF *)
-        destruct w; cbn in H2, H3; setoid_rewrite Heqt in H2;
-          setoid_rewrite Heqt in H3.
+        destruct w.
         * (* RetF, Pure *)
-          destruct (H2 _ _ TR); dependent destruction TR.
+          destruct (H2 _ _ TR_); dependent destruction TR_.
           -- apply AFNowIndDone with x0; auto.
           -- destruct H1.
              apply can_step_not_done in H1.
              inv H1.
         * (* RetF, Obs e v *)
-          destruct (H2 _ _ TR); dependent destruction TR.
+          destruct (H2 _ _ TR_); dependent destruction TR_.
           -- apply AFNowIndFinish with x0; auto.
           -- destruct H1.
              apply can_step_not_done in H1.
              inv H1.
-        * (* RetF, Done *) dependent destruction TR.
-        * (* RetF, Finish *) dependent destruction TR.
-      + (* Br b n k *)
-        apply AFNowIndBr with b n k; auto.
-        * apply ktrans_not_done with (Br b n k) t' w'; auto.
-        * destruct b.
-          -- (* BrS *)
-            intros i Hs.
-            apply ktrans_brS in TR as (? & ? & -> & ?).
-            apply H3; cbn.
-            rewrite Heqt.
-            apply ktrans_brS.
-            exists i; auto.
+        * (* RetF, Done *) dependent destruction TR_.
+        * (* RetF, Finish *) dependent destruction TR_.
+      + (* BrS n k *)
+        apply AFNowIndBrS with n k; auto.
+        * apply ktrans_not_done with (BrS n k) t_ w_; auto.
+        * intros i.
+          apply H3.
+          apply KtransBrS with i; auto.
+          apply ktrans_not_done with (BrS n k) t_ w_; auto.
+      + (* BrD n k *)
+        
+            exists x.
+            exists t', w'.
+            admit.
           -- (* BrD *)
-            intros i (t_ & w_ & TR_).
+            apply ktrans_brD in TR.
+            ++ destruct TR.
+               exists x.
+               exists t', w'; auto.
+        * (* AF *)
+          intros i Hd.
+          destruct b.
+          ++ admit.
+          ++ (* BrD *)           
+            apply ktrans_brD in TR as (j & TR).
+            apply H3.
+            cbn.
+            rewrite Heqt.
+            apply ktrans_brD.
+            
+            
+              intros i (t_ & w_ & TR_).
             assert(TR': [t, w] ↦ [t_, w_]).
             { cbn; rewrite Heqt; apply ktrans_brD; exists i; auto. }
             cbn in TR_, TR', H2, H3.
